Rejig Broadcast to build upon Execution

src/Broadcast.thy
@@ -3,52 +3,10 @@ section\<open>Implementation of Causal Broadcast Protocol\<close>
 theory
   Broadcast
 imports
+  Execution
   Network
   Util
 begin
-
-subsection\<open>Non-determinism of users and networks\<close>
-
-locale executions =
-  fixes initial   :: "'nodeid \<Rightarrow> 'state"
-    and valid_msg :: "'nodeid \<Rightarrow> 'state \<Rightarrow> 'msg set"
-    and send_msg  :: "'nodeid \<Rightarrow> 'msg \<Rightarrow> 'state \<Rightarrow> 'state"
-    and recv_msg  :: "'nodeid \<Rightarrow> 'msg \<Rightarrow> 'state \<Rightarrow> 'state"
-
-definition (in executions) user_step :: "('nodeid \<Rightarrow> 'state \<times> 'msg set) \<Rightarrow> ('nodeid \<Rightarrow> 'state \<times> 'msg set)" where
-  "user_step conf \<equiv>
-     let sender = SOME node::'nodeid. True;
-         (state, msgs) = conf sender in
-     if valid_msg sender state \<noteq> {} then
-       let msg = SOME msg. msg \<in> valid_msg sender state in
-         conf(sender := (send_msg sender msg state, insert msg msgs))
-     else conf"
-
-definition (in executions) network_step :: "('nodeid \<Rightarrow> 'state \<times> 'msg set) \<Rightarrow> ('nodeid \<Rightarrow> 'state \<times> 'msg set)" where
-  "network_step conf \<equiv>
-     let sender = SOME node::'nodeid. True;
-         recipient = SOME node::'nodeid. node \<noteq> sender in
-     if snd (conf sender) \<noteq> {} then
-       let msg = SOME msg. msg \<in> snd (conf sender);
-           (state, msgs) = conf recipient
-       in conf(recipient := (recv_msg recipient msg state, msgs))
-     else conf"
-
-definition (in executions) take_step :: "('nodeid \<Rightarrow> 'state \<times> 'msg set) \<Rightarrow> ('nodeid \<Rightarrow> 'state \<times> 'msg set)" where
-  "take_step \<equiv> SOME step. step \<in> {user_step, network_step}"
-
-inductive (in executions) execution :: "('nodeid \<Rightarrow> 'state \<times> 'msg set) \<Rightarrow> bool" where
-  "execution (\<lambda>n. (initial n, {}))" |
-  "\<lbrakk> execution conf; take_step conf = conf' \<rbrakk> \<Longrightarrow> execution conf'"
-
-(* I think this definition is equivalent, but makes the non-deterministic choices less explicit:
-inductive (in executions) execution :: "('nodeid \<Rightarrow> 'state \<times> 'msg set) \<Rightarrow> bool" where
-  "execution (\<lambda>n. (initial n, {}))" |
-  "\<lbrakk> execution conf; conf sender = (state, msgs); msg \<in> valid_msg state; state' = send_msg msg state \<rbrakk>
-       \<Longrightarrow> execution (conf(sender := (state', insert msg msgs)))" |
-  "\<lbrakk> execution conf; conf recver = (state, msgs); msg \<in> snd (conf sender); state' = recv_msg msg state \<rbrakk>
-       \<Longrightarrow> execution (conf(recver := (state', msgs)))"
-*)
 
 subsection\<open>Causal broadcasts using vector timestamps\<close>
 
@@ -59,13 +17,13 @@ record ('nodeid, 'op) message =
   msg_deps :: "'nodeid \<Rightarrow> nat"
   msg_op   :: "'op"
 
-type_synonym ('nodeid, 'op) node_state = "('nodeid, 'op) message event list"
+type_synonym ('nodeid, 'op) node_state = "(('nodeid, 'op) message event, unit) node"
 
 definition broadcasts :: "('nodeid, 'op) node_state \<Rightarrow> ('nodeid, 'op) message list" where
-  "broadcasts state \<equiv> List.map_filter (\<lambda>e. case e of Broadcast m \<Rightarrow> Some m | _ \<Rightarrow> None) state"
+  "broadcasts state \<equiv> List.map_filter (\<lambda>e. case e of Broadcast m \<Rightarrow> Some m | _ \<Rightarrow> None) (fst state)"
 
 definition deliveries :: "('nodeid, 'op) node_state \<Rightarrow> ('nodeid, 'op) message list" where
-  "deliveries state \<equiv> List.map_filter (\<lambda>e. case e of Deliver m \<Rightarrow> Some m | _ \<Rightarrow> None) state"
+  "deliveries state \<equiv> List.map_filter (\<lambda>e. case e of Deliver m \<Rightarrow> Some m | _ \<Rightarrow> None) (fst state)"
 
 definition causal_deps :: "('nodeid, 'op) node_state \<Rightarrow> 'nodeid \<Rightarrow> nat" where
   "causal_deps state \<equiv> foldl
@@ -90,396 +48,70 @@ definition valid_msgs :: "(('nodeid, 'op) node_state \<Rightarrow> 'op set) \<Ri
               msg_op   = oper\<rparr>
      ) ` valid_ops state"
 
-definition protocol_send :: "'nodeid \<Rightarrow> ('nodeid, 'op) message \<Rightarrow> ('nodeid, 'op) node_state \<Rightarrow> ('nodeid, 'op) node_state" where
-  "protocol_send sender msg hist \<equiv> hist @ [Broadcast msg, Deliver msg]"
+definition protocol_send ::
+  "'nodeid \<Rightarrow> ('nodeid, 'op) node_state \<Rightarrow> ('nodeid, 'op) message \<Rightarrow> ('nodeid, 'op) node_state" where
+  "protocol_send sender state msg \<equiv> ([Broadcast msg, Deliver msg], ())"
 
-definition protocol_recv :: "'nodeid \<Rightarrow> ('nodeid, 'op) message \<Rightarrow> ('nodeid, 'op) node_state \<Rightarrow> ('nodeid, 'op) node_state" where
-  "protocol_recv recipient msg hist \<equiv>
-     if causally_ready hist msg then hist @ [Deliver msg] else hist"
+definition protocol_recv ::
+  "'nodeid \<Rightarrow> ('nodeid, 'op) node_state \<Rightarrow> ('nodeid, 'op) message \<Rightarrow> ('nodeid, 'op) node_state" where
+  "protocol_recv recipient state msg \<equiv>
+     if causally_ready state msg then ([Deliver msg], ()) else ([], ())"
 
-type_synonym 'op configuration = "nat \<Rightarrow> (nat, 'op) node_state \<times> (nat, 'op) message set"
-
-locale cbcast_protocol_base = executions "\<lambda>n. []" _ protocol_send protocol_recv +
+locale cbcast_protocol_base = executions "\<lambda>n. ()" valid_msg protocol_send protocol_recv
+  for valid_msg :: "nat \<Rightarrow> (nat, 'op) message event list \<times> unit \<Rightarrow> (nat, 'op) message set" +
   fixes valid_ops :: "(nat, 'op) node_state \<Rightarrow> 'op set"
 
-locale cbcast_protocol = cbcast_protocol_base "valid_msgs valid_ops" +
-  fixes config :: "'a configuration"
+locale cbcast_protocol = cbcast_protocol_base "valid_msgs valid_ops" valid_ops
+  for valid_ops :: "(nat, 'op) message event list \<times> unit \<Rightarrow> 'op set" +
+  fixes config :: "(nat, (nat, 'op) message, (nat, 'op) message event, unit) system"
   assumes valid_execution: "execution config"
 
-definition (in cbcast_protocol) history :: "nat \<Rightarrow> (nat, 'a) message event list" where
-  "history i \<equiv> fst (config i)"
+definition (in cbcast_protocol) history :: "nat \<Rightarrow> (nat, 'op) message event list" where
+  "history i \<equiv> fst (snd config i)"
 
-definition (in cbcast_protocol) broadcasts :: "nat \<Rightarrow> (nat, 'a) message list" where
+definition (in cbcast_protocol) all_messages :: "(nat, 'op) message set" where
+  "all_messages \<equiv> fst config"
+
+definition (in cbcast_protocol) broadcasts :: "nat \<Rightarrow> (nat, 'op) message list" where
   "broadcasts i \<equiv> List.map_filter (\<lambda>e. case e of Broadcast m \<Rightarrow> Some m | _ \<Rightarrow> None) (history i)"
 
-definition (in cbcast_protocol) deliveries :: "nat \<Rightarrow> (nat, 'a) message list" where
+definition (in cbcast_protocol) deliveries :: "nat \<Rightarrow> (nat, 'op) message list" where
   "deliveries i \<equiv> List.map_filter (\<lambda>e. case e of Deliver m \<Rightarrow> Some m | _ \<Rightarrow> None) (history i)"
 
 
-subsection\<open>Proof that this protocol satisfies the causal axiom\<close>
-
-definition (in cbcast_protocol) config_evolution :: "'a configuration \<Rightarrow> 'a configuration list \<Rightarrow> bool" where
-  "config_evolution c cs \<equiv>
-     cs \<noteq> [] \<and>
-     hd cs = (\<lambda>n. ([], {})) \<and>
-     last cs = c \<and>
-     (\<forall>x \<in> set cs. execution x) \<and>
-     (\<forall>pre x y suf. cs = pre@x#y#suf \<longrightarrow> user_step x = y \<or> network_step x = y)"
-
-lemma (in cbcast_protocol) config_evolution_drop_last:
-  assumes "config_evolution c2 (confs@[c1,c2])"
-  shows "config_evolution c1 (confs@[c1])"
-  using assms apply(simp add: config_evolution_def)
-  apply(erule conjE)+
-  apply(rule conjI)
-  apply(simp add: list_head_unaffected)
-  apply(metis (no_types, lifting) append.assoc append.simps(2) self_append_conv2)
-done
-
-lemma (in cbcast_protocol) config_evolution_drop_last2:
-  assumes "config_evolution (last cs) cs"
-    and "length cs > 1"
-  shows "config_evolution (last (butlast cs)) (butlast cs)"
-  using assms apply -
-  apply(subgoal_tac "\<exists>c1 c2 confs. cs = confs@[c1,c2]")
-  apply(erule exE)+
-  apply(simp add: butlast_append config_evolution_drop_last)
-  using list_two_at_end apply blast
-done
-
-lemma (in cbcast_protocol) config_evolution_exists:
-  assumes "execution conf"
-  shows "\<exists>confs. config_evolution conf confs"
-  using assms unfolding config_evolution_def
-  apply(induction rule: execution.induct)
-  apply(rule_tac x="[\<lambda>a. ([], {})]" in exI)
-  apply(simp add: execution.intros(1))
-  apply(erule exE)
-  apply(rule_tac x="confs@[conf']" in exI, clarsimp)
-  apply(rule conjI)
-  using execution.intros(2) last_in_set apply blast
-  apply(rule allI)+
-  apply(subgoal_tac "take_step \<in> {user_step, network_step}") defer
-  apply(rule choose_set_memb, simp, simp add: take_step_def)
-  apply(simp, erule disjE, clarsimp)
-  apply(case_tac suf, force)
-  apply(metis (no_types, lifting) butlast.simps(2) butlast_append butlast_snoc list.simps(3))
-  apply(clarsimp, case_tac suf, force)
-  apply(metis (no_types, lifting) butlast.simps(2) butlast_append butlast_snoc list.simps(3))
-done
-
-lemma (in cbcast_protocol) config_evolution_fold:
-  assumes "execution conf"
-  shows "\<exists>steps. conf = fold (op \<circ>) steps id (\<lambda>n. ([], {}))"
-  using assms unfolding config_evolution_def
-  apply(induction rule: execution.induct)
-  apply(rule_tac x="[]" in exI, simp)
-  apply(erule exE)
-  apply(rule_tac x="steps@[take_step]" in exI, simp)
-done
-
-lemma (in cbcast_protocol) config_evolution_butlast:
-  assumes "config_evolution conf (confs@[conf])"
-    and "conf \<noteq> (\<lambda>n. ([], {}))"
-  shows "config_evolution (last confs) confs"
-  using assms unfolding config_evolution_def apply clarsimp
-  apply(rule conjI, force)
-  apply(rule conjI)
-  apply(metis (mono_tags, lifting) hd_append list.sel(1))
-  apply clarsimp
-  apply(erule_tac x=pre in allE, erule_tac x=x in allE, erule_tac x=y in allE)
-  apply blast
-done
-
-lemma (in cbcast_protocol) user_step_effect:
-  assumes "user_step before = after"
-    and "before \<noteq> after"
-  shows "\<exists>i es msg msgs. msgs = valid_msgs valid_ops i (fst (before i)) \<and> msgs \<noteq> {} \<and> msg \<in> msgs \<and>
-           after = before(i := (protocol_send i msg (fst (before i)), insert msg (snd (before i))))"
-  using assms
-  apply(simp add: user_step_def)
-  apply(erule unpack_let)
-  apply(simp add: case_prod_beta split: if_split_asm)
-  apply(erule unpack_let)
-  apply(rule_tac x=sender in exI)
-  apply(rule conjI, simp)
-  apply(rule_tac x=msg in exI)
-  apply(rule conjI, simp add: some_set_memb, simp)
-done
-
-lemma (in cbcast_protocol) network_step_effect:
-  assumes "network_step before = after"
-    and "before \<noteq> after"
-  shows "\<exists>sender recipient es msg msgs. msgs = snd (before sender) \<and> msgs \<noteq> {} \<and> msg \<in> msgs \<and>
-    after = before(recipient := (protocol_recv recipient msg (fst (before recipient)), snd (before recipient)))"
-  using assms
-  apply(simp add: network_step_def)
-  apply(erule unpack_let)
-  apply(erule unpack_let)
-  apply(simp add: case_prod_beta split: if_split_asm)
-  apply(subgoal_tac "\<exists>msg. msg = (SOME msg. msg \<in> snd (before sender))", erule exE)
-  apply(rule_tac x=sender in exI, simp)
-  apply(rule_tac x=recipient in exI, rule_tac x=msg in exI, simp)
-  apply(meson ex_in_conv some_eq_ex)
-  using some_set_memb apply blast
-done
-
-lemma (in cbcast_protocol) history_append:
-  assumes "config_evolution conf confs"
-  and "\<exists>suf. pre@x#y#suf = confs"
-  shows "(user_step x = y \<or> network_step x = y) \<and>
-      (\<exists>i es. fst (x i) @ es = fst (y i) \<and> (\<forall>j::nat. i\<noteq>j \<longrightarrow> fst (x j) = fst (y j)))"
-  using assms apply(simp add: config_evolution_def)
-  apply(erule conjE)+
-  apply(erule_tac x=pre in allE, erule_tac x=x in allE, erule_tac x=y in allE)
-  apply(subgoal_tac "user_step x = y \<or> network_step x = y \<Longrightarrow>
-       \<exists>i. (\<exists>es. fst (x i) @ es = fst (y i)) \<and> (\<forall>j. i \<noteq> j \<longrightarrow> fst (x j) = fst (y j))")
-  apply blast
-  apply(case_tac "x=y")
-  apply(rule_tac x=0 in exI, simp)
-  apply(erule disjE)
-  apply(drule user_step_effect, assumption)
-  apply(metis protocol_send_def fst_conv fun_upd_other fun_upd_same)
-  apply(drule network_step_effect, assumption)
-  apply(metis (no_types, lifting) protocol_recv_def fst_conv append_Nil2 fun_upd_other fun_upd_same)
-done
-
-lemma (in cbcast_protocol) history_nonempty:
-  assumes "execution conf"
-  and "evt \<in> set (fst (conf i))"
-  shows "\<exists>confs. config_evolution conf confs \<and> length confs > 1"
-  using assms apply -
-  apply(drule config_evolution_exists, erule exE)
-  apply(rule_tac x=confs in exI, clarsimp)
-  apply(simp add: config_evolution_def)
-  apply(erule conjE)+
-  apply(subgoal_tac "length confs \<le> 1 \<Longrightarrow> False", fastforce)
-  apply(metis empty_iff empty_set fst_conv last_ConsL le_less length_0_conv less_one list_head_length_one)
-done
-
-lemma (in cbcast_protocol) history_nonempty2:
-  assumes "execution conf"
-  and "config_evolution conf confs"
-  and "evt \<in> set (fst (conf i))"
-  shows "\<exists>pre c. confs = pre @ [c, conf]"
-  using assms apply(simp add: config_evolution_def)
-  apply(erule conjE)+
-  apply(subgoal_tac "butlast confs \<noteq> []")
-  apply(rule_tac x="butlast (butlast confs)" in exI)
-  apply(rule_tac x="last (butlast confs)" in exI)
-  apply(metis append_assoc append_butlast_last_id butlast.simps(2) last.simps list.simps(3))
-  apply(subgoal_tac "butlast confs = [] \<Longrightarrow> False", fastforce)
-  apply(subgoal_tac "confs = [\<lambda>n. ([], {})]")
-  apply(metis empty_iff empty_set fst_conv last_ConsL)
-  apply(metis append_butlast_last_id append_self_conv2 list.sel(1))
-done
-
-lemma (in cbcast_protocol) history_append_simp:
-  assumes "conf' = conf(i := (fst (conf i) @ xs, insert msg (snd (conf i))))"
-  shows "fst (conf i) @ xs = fst (conf' i)"
-using assms by simp
-
-lemma (in cbcast_protocol) history_fold:
-  assumes "execution conf"
-  shows "\<exists>steps. conf = fold (op \<circ>) (map fst steps) id (\<lambda>n. ([], {})) \<and>
-         fst (conf i) = foldl (op @) [] (map snd steps)"
-  using assms
-  apply(induction rule: execution.induct)
-  apply(rule_tac x="[]" in exI, simp)
-  apply(erule exE)
-  apply(case_tac "conf=conf'", rule_tac x="steps" in exI, clarsimp)
-  apply(subgoal_tac "take_step \<in> {user_step, network_step}") defer
-  apply(rule choose_set_memb, simp, simp add: take_step_def)
-  apply(simp, erule disjE, simp)
-  apply(frule user_step_effect, assumption, (erule exE)+, (erule conjE)+)
-  apply(subst (asm) protocol_send_def)
-  apply(case_tac "i=ia")
-  apply(rule_tac x="steps@[(take_step, [Broadcast msg, Deliver msg])]" in exI, simp)
-  apply(rule_tac x="steps@[(take_step, [])]" in exI, simp)
-  apply(simp, frule network_step_effect, assumption, (erule exE)+, (erule conjE)+)
-  apply(subst (asm) protocol_recv_def)
-  apply(case_tac "i = recipient")
-  apply(case_tac "causally_ready (fst (conf recipient)) msg")
-  apply(rule_tac x="steps@[(take_step, [Deliver msg])]" in exI, simp)
-  apply(rule_tac x="steps@[(take_step, [])]" in exI, simp)
-  apply(rule_tac x="steps@[(take_step, [])]" in exI, simp)
-done
-
-lemma (in cbcast_protocol) event_creation:
-  assumes "execution conf"
-    and "evt \<in> set (fst (conf i))"
-  shows "\<exists>before after es. evt \<in> set es \<and> before \<noteq> after \<and>
-    (user_step before = after \<or> network_step before = after) \<and>
-    fst (before i) @ es = fst (after i)"
-  using assms
-  apply(induction rule: execution.induct, simp)
-  apply(case_tac "conf=conf'", simp)
-  apply(subgoal_tac "take_step \<in> {user_step, network_step}") defer
-  apply(rule choose_set_memb, simp, simp add: take_step_def)
-  apply(simp, erule disjE, simp)
-  apply(frule user_step_effect, assumption, (erule exE)+, (erule conjE)+)
-  apply(subst (asm) protocol_send_def)
-  apply(case_tac "i=ia")
-  apply(case_tac "evt \<in> {Broadcast msg, Deliver msg}")
-  apply(rule_tac x=conf in exI, rule_tac x=conf' in exI)
-  apply(rule_tac x="[Broadcast msg, Deliver msg]" in exI, simp)
-  apply(subgoal_tac "evt \<in> set (fst (conf i))", simp)
-  apply(subgoal_tac "fst (conf ia) @ [Broadcast msg, Deliver msg] = fst (conf' ia)")
-  apply(metis UnE empty_set list.simps(15) set_append, simp, simp)
-  apply(case_tac "conf=conf'", simp, simp)
-  apply(frule network_step_effect, assumption, (erule exE)+, (erule conjE)+)
-  apply(subst (asm) protocol_recv_def)
-  apply(case_tac "i = recipient")
-  apply(case_tac "causally_ready (fst (conf recipient)) msg")
-  apply(case_tac "evt = Deliver msg")
-  apply(rule_tac x=conf in exI, rule_tac x=conf' in exI)
-  apply(rule_tac x="[Deliver msg]" in exI, simp)
-  apply(subgoal_tac "evt \<in> set (fst (conf i))", simp)
-  apply(subgoal_tac "fst (conf recipient) @ [Deliver msg] = fst (conf' recipient)")
-  apply(metis UnE empty_iff empty_set set_ConsD set_append)
-  apply simp+
-done
-
-lemma broadcast_in_set:
-  assumes "broadcasts hist = pre @ [msg] @ suf"
-    shows "Broadcast msg \<in> set hist"
-  using assms apply -
-  apply(induction hist arbitrary: pre suf rule: rev_induct)
-  apply(simp add: broadcasts_def List.map_filter_def)
-  apply(case_tac x, case_tac "x1=msg", simp)
-  apply(erule_tac x=pre in meta_allE)
-  apply(erule_tac x="butlast suf" in meta_allE)
-  apply(simp add: broadcasts_def List.map_filter_def)
-  apply(metis (no_types, lifting) butlast.simps(2) butlast_append butlast_snoc last_ConsL last_appendR list.simps(3))
-  apply(erule_tac x=pre in meta_allE, erule_tac x=suf in meta_allE)
-  apply(simp add: broadcasts_def List.map_filter_def)
-done
+subsection\<open>Proof that this protocol satisfies the causal network assumptions\<close>
 
 lemma (in cbcast_protocol) broadcast_node_id:
   assumes "Broadcast msg \<in> set (history i)"
     and "msg_id msg = (j, seq)"
   shows "i = j"
   using assms valid_execution apply(simp add: history_def)
-  apply(drule event_creation, simp)
-  apply((erule exE)+, (erule conjE)+, erule disjE)
-  apply(subgoal_tac "msg_id msg = next_msgid i (fst (before i))")
+  apply(drule event_origin, simp)
+  apply((erule exE)+, (erule conjE)+)
+  apply(subgoal_tac "msg_id msg = next_msgid i (snd before i)")
   apply(simp add: next_msgid_def)
-  apply(simp add: user_step_def)
-  apply(erule let_some_elim, simp+)
-  apply(simp add: case_prod_beta split: if_split_asm)
-  apply(erule let_some_elim, blast)
-  apply(case_tac "node=i", case_tac "msga=msg")
-  apply(clarsimp simp add: valid_msgs_def)
-  apply(metis event.distinct(1) event.inject(1) fst_conv fun_upd_same nat.simps(3)
-    protocol_send_def same_append_eq set_ConsD trivial_network.broadcasts_unique)
-  apply auto[1]
-  apply(simp add: network_step_def)
-  apply(erule let_some_elim, simp, erule let_some_elim, presburger)
-  apply(simp add: case_prod_beta protocol_recv_def split: if_split_asm)
-  apply(erule let_some_elim, blast)
-  apply(simp split: if_split_asm)
-  apply(case_tac "nodea=i", case_tac "msga=msg")
-  apply auto
-done
-
-lemma (in cbcast_protocol) config_evolution_append:
-  assumes "config_evolution conf (cs1 @ step # cs2)"
-  shows "\<exists>suf. fst (step i) @ suf = fst (conf i)"
-  using assms apply -
-  apply(induction cs2 arbitrary: conf rule: rev_induct)
-  apply(rule_tac x="[]" in exI)
-  apply(metis (mono_tags, lifting) config_evolution_def last_snoc self_append_conv)
-  apply(subgoal_tac "x=conf") defer
-  apply(metis (mono_tags, lifting) config_evolution_def last.simps last_append
-    list.distinct(1) snoc_eq_iff_butlast)
-  apply clarsimp
-  apply(insert config_evolution_drop_last2)
-  apply(erule_tac x="cs1 @ step # xs @ [conf]" in meta_allE)
-  apply(simp add: butlast_append)
-  apply(case_tac "xs=[]")
-  apply(erule_tac x="step" in meta_allE, clarsimp)
-  apply(insert history_append)
-  apply(erule_tac x=conf in meta_allE)
-  apply(erule_tac x="cs1 @ [step, conf]" in meta_allE)
-  apply(erule_tac x=cs1 in meta_allE)
-  apply(erule_tac x=step in meta_allE)
-  apply(erule_tac x=conf in meta_allE, clarsimp)
-  apply(case_tac "i=ia")
-  apply(rule_tac x="es" in exI, simp)
-  apply(rule_tac x="[]" in exI, simp)
-  apply(erule_tac x="last xs" in meta_allE)
-  apply(erule_tac x="conf" in meta_allE)
-  apply(erule_tac x="cs1 @ step # xs @ [conf]" in meta_allE, clarsimp)
-  apply(erule_tac x="cs1 @ step # butlast xs" in meta_allE)
-  apply(erule_tac x="last xs" in meta_allE)
-  apply(erule_tac x="conf" in meta_allE)
-  apply(subgoal_tac "\<exists>suf. cs1 @ step # butlast xs @ last xs # conf # suf = cs1 @ step # xs @ [conf]")
-  apply(clarsimp)
-  apply(case_tac "i=ia")
-  apply(rule_tac x="suf@es" in exI, metis append.assoc)
-  apply(rule_tac x="suf" in exI, simp)
-  apply(rule_tac x="[]" in exI, simp)
-done
-
-lemma (in cbcast_protocol) broadcast_origin:
-  assumes "config_evolution conf confs"
-    and "fst (conf i) = pre @ [Broadcast msg] @ suf"
-    (*and "Broadcast msg \<notin> set suf"*)
-  shows "\<exists>before after msgs. msgs = valid_msgs valid_ops i (fst (before i)) \<and> msgs \<noteq> {} \<and> msg \<in> msgs \<and>
-           after = before(i := (fst (before i) @ [Broadcast msg, Deliver msg], insert msg (snd (before i))))"
-  using assms apply -
-  apply(insert history_append, erule_tac x=conf in meta_allE, erule_tac x=confs in meta_allE)
-  apply(induction confs arbitrary: conf suf rule: rev_induct)
-  apply(simp add: config_evolution_def)
-  apply(case_tac "xs=[]")
-  using config_evolution_def apply fastforce
-  apply(simp)
-  apply(erule_tac x="butlast xs" in meta_allE)
-  apply(erule_tac x="last xs" in meta_allE)
-  apply(erule_tac x="last xs" in meta_allE)
-  apply(erule_tac x="x" in meta_allE)
-  apply(subgoal_tac "\<exists>suf. xs @ [x] = butlast xs @ last xs # x # suf") defer
-  apply(metis (no_types, lifting) append_butlast_last_id append_eq_append_conv2
-    butlast.simps(2) last_ConsL last_ConsR list.simps(3))
-  apply(clarsimp)
-  apply(case_tac "i=ia")
-  apply(case_tac "Broadcast msg \<in> set(es)")
-  apply(rule_tac x="last xs" in exI, clarsimp)
   apply(erule disjE)
-  apply(simp add: user_step_def)
-  apply(erule let_some_elim, simp+)
-  apply(simp add: case_prod_beta split: if_split_asm)
-  apply(erule let_some_elim, blast)
-  apply(case_tac "node=i", case_tac "msga=msg", blast)
-  apply(simp add: protocol_send_def)
-  apply auto[1]
-  apply(metis (no_types, lifting) append_self_conv ex_in_conv fun_upd_def set_empty)
-  apply(simp add: network_step_def)
-  apply(erule let_some_elim, simp, erule let_some_elim, presburger)
-  apply(simp add: case_prod_beta protocol_recv_def split: if_split_asm)
-  apply(erule let_some_elim, blast)
-  apply(simp split: if_split_asm)
-  apply(case_tac "nodea=i", case_tac "msga=msg")
-  apply auto[1]
-  apply auto[1]
-  apply(metis (no_types, lifting) append_self_conv fst_conv fun_upd_same not_Cons_self2)
-  apply(insert config_evolution_append)
-  apply(erule_tac x="conf" in meta_allE)
-  apply(erule_tac x="butlast xs" in meta_allE)
-  apply(erule_tac x="last xs" in meta_allE)
-  apply(erule_tac x="x # sufa" in meta_allE)
-  apply(erule_tac x="i" in meta_allE, clarsimp)
-  apply(erule_tac x="drop_final (length sufb) suf" in meta_allE)
-  apply(subgoal_tac "config_evolution (last xs) xs")
-  apply(subgoal_tac "fst (last xs i) = pre @ Broadcast msg # drop_final (length sufb) suf")
-  apply(insert history_append)
-  apply(erule_tac x="last xs" in meta_allE, erule_tac x=xs in meta_allE, simp)
-  
-  oops
+  apply(simp add: send_step_def case_prod_beta)
+  apply(erule unpack_let)+
+  apply(simp add: case_prod_beta protocol_send_def split: if_split_asm)
+  apply(erule unpack_let)
+  apply(subgoal_tac "sender=i") prefer 2 apply force
+  apply(subgoal_tac "fst (snd after i) = fst (snd before i) @ [Broadcast msga, Deliver msga]")
+  prefer 2 apply force
+  apply(subgoal_tac "msga=msg") prefer 2 apply simp
+  apply(subgoal_tac "msg \<in> valid_msgs valid_ops i (snd before i)")
+  prefer 2 apply(simp add: some_set_memb)
+  apply(simp add: valid_msgs_def, force)
+  apply(simp add: recv_step_def protocol_recv_def case_prod_beta split: if_split_asm)
+  apply(erule unpack_let)+
+  apply(subgoal_tac "recipient=i")
+  apply force+
+done
+
 
 lemma (in cbcast_protocol) broadcast_msg_id:
-  assumes "history i = pre @ [Broadcast msg] @ suf"
-    shows "msg_id msg = (i, Suc (length (Broadcast.broadcasts pre)))"
+  assumes "broadcasts i = pre @ [msg] @ suf"
+    shows "msg_id msg = (i, Suc (length pre))"
   oops
 
 context cbcast_protocol begin
